\documentclass[10pt, letterpaper, twoside]{article}
\usepackage[T1]{fontenc}
\usepackage{garamond}
\usepackage{mathtools}
\usepackage{geometry}
\geometry{margin=1in}

\newcommand{\pd}[2]{\frac{\partial#1}{\partial#2}}

\title{Nondimensionalization of Haseloff et al. 2018}
\author{Pierce Hunter}
\date{1/24/2019}

\begin{document}
	\maketitle
	
	\section{Nondimensionalization of Velocity Equations}
	Nondimensionalizing the equations in terms of dimensional scales (this section will not yet try write the scales in terms of parameters)\\
	Here I use:
	\begin{gather*}
		y = \left[z\right]Y \qquad
		z = \left[z\right]Z\\
		u = \left[u\right]U \qquad
		v = \left[v\right]V \qquad
		w = \left[v\right]W\\
		\eta = \left[\eta\right]\mu \qquad
		p = \left[p\right]P \qquad
		s' = \left[s'\right]S'
	\end{gather*}
	The convention I used here is to provide the equation number when it matches the same equation in Haseloff's paper. If the equation doesn't match an equation in Haseloff, but I plan to resolve the differences later in the notes I will denote that with primes.
	\subsection{2 $ \rightarrow $ 22}
	\begin{gather*}
		\pd{}{y}\left(\eta\pd{u}{y}\right) + \pd{}{z}\left(\eta\pd{u}{z}\right) = 0 \tag{2} \\
		\frac{1}{\left[z\right]}\pd{}{Y}\left(\left[\eta\right]\mu\frac{\left[u\right]}{\left[z\right]}\pd{U}{Y}\right) + \frac{1}{\left[z\right]}\pd{}{Z}\left(\left[\eta\right]\mu\frac{\left[u\right]}{\left[z\right]}\pd{U}{Z}\right) = 0\\
		\frac{\left[\eta\right]\left[u\right]}{\left[z\right]^2}\left[\pd{}{Y}\left(\mu\pd{U}{Y}\right) + \pd{}{Z}\left(\mu\pd{U}{Z}\right)\right] = 0\\
		\pd{}{Y}\left(\mu\pd{U}{Y}\right) + \pd{}{Z}\left(\mu\pd{U}{Z}\right) = 0 \tag{22}
	\end{gather*}
	\subsection{3a $ \rightarrow $ 23a}
	\begin{gather*}
		\pd{}{y}\left(2\eta\pd{v}{y}\right) + \pd{}{z}\left[\eta\left(\pd{v}{z}+\pd{w}{y}\right)\right] - \pd{p}{y} = 0 \tag{3a} \\
		\frac{1}{\left[z\right]}\pd{}{Y}\left(2\left[\eta\right]\mu\frac{\left[v\right]}{\left[z\right]}\pd{V}{Y}\right) + \frac{1}{\left[z\right]}\pd{}{Z}\left[\left[\eta\right]\mu\frac{\left[v\right]}{\left[z\right]}\left(\pd{V}{Z}+\pd{W}{Y}\right)\right] - \frac{\left[p\right]}{\left[z\right]}\pd{P}{Y} = 0\\
		\frac{\left[\eta\right]\left[v\right]}{\left[z\right]^2}\pd{}{Y}\left(2\mu\pd{V}{Y}\right) + \frac{\left[\eta\right]\left[v\right]}{\left[z\right]^2}\pd{}{Z}\left[\mu\left(\pd{V}{Z}+\pd{W}{Y}\right)\right] - \frac{\left[p\right]}{\left[z\right]}\pd{P}{Y} = 0 \tag{3a$'$}
	\end{gather*}
	\subsection{3b $ \rightarrow $ 23b}
	\begin{gather*}
		\pd{}{y}\left[\eta\left(\pd{v}{z}+\pd{w}{y}\right)\right] + \pd{}{z}\left(2\eta\pd{w}{z}\right) - \pd{p}{z} = 0 \tag{3b} \\
		\frac{1}{\left[z\right]}\pd{}{Y}\left[\left[\eta\right]\mu\frac{\left[v\right]}{\left[z\right]}\left(\pd{V}{Z}+\pd{W}{Y}\right)\right] + \frac{1}{\left[z\right]}\pd{}{Z}\left(2\left[\eta\right]\mu\frac{\left[v\right]}{\left[z\right]}\pd{W}{Z}\right) - \frac{\left[p\right]}{\left[z\right]}\pd{P}{Z} = 0\\
		\frac{\left[\eta\right]\left[v\right]}{\left[z\right]^2}\pd{}{Y}\left[\mu\left(\pd{V}{Z}+\pd{W}{Y}\right)\right] + \frac{\left[\eta\right]\left[v\right]}{\left[z\right]^2}\pd{}{Z}\left(2\mu\pd{W}{Z}\right) - \frac{\left[p\right]}{\left[z\right]}\pd{P}{Z} = 0 \tag{3b$'$}
	\end{gather*}
	\subsection{3c $ \rightarrow $ 23c}
	\begin{gather*}
		\pd{v}{y} + \pd{w}{z} = 0 \tag{3c} \\
		\frac{\left[v\right]}{\left[z\right]}\pd{V}{Y} + \frac{\left[v\right]}{\left[z\right]}\pd{W}{Z} = 0\\
		\pd{V}{Y} + \pd{W}{Z} = 0 \tag{23c}
	\end{gather*}
	\subsection{4 $ \rightarrow $ 24}
	\begin{gather*}
		\eta = \frac{A^{-1/n}}{2^{1/n}}\left[\left|\pd{u}{y}\right|^2 + \left|\pd{u}{z}\right|^2 + \left|\pd{v}{z} + \pd{w}{y}\right|^2 + 2\left|\pd{v}{y}\right|^2 + 2\left|\pd{w}{z}\right|^2\right]^{\frac{1-n}{2n}} \tag{4} \\
		\frac{A^{-1/n}}{2^{1/n}}\left[\frac{\left[u\right]^2}{\left[z\right]^2}\left(\left|\pd{U}{Y}\right|^2 + \left|\pd{U}{Z}\right|^2\right) + \frac{\left[v\right]^2}{\left[z\right]^2}\left(\left|\pd{V}{Z} + \pd{W}{Y}\right|^2 + 2\left|\pd{V}{Y}\right|^2 + 2\left|\pd{W}{Z}\right|^2\right)\right]^{\frac{1-n}{2n}}\\
		\frac{A^{-1/n}}{2^{1/n}}\left(\frac{\left[u\right]}{\left[z\right]}\right)^{\frac{1-n}{n}}\left[\left|\pd{U}{Y}\right|^2 + \left|\pd{U}{Z}\right|^2 + \frac{\left[v\right]^2}{\left[u\right]^2}\left(\left|\pd{V}{Z} + \pd{W}{Y}\right|^2 + 2\left|\pd{V}{Y}\right|^2 + 2\left|\pd{W}{Z}\right|^2\right)\right]^{\frac{1-n}{2n}} \tag{4$'$}
	\end{gather*}
	\subsection{5 $ \rightarrow $ 25}
	Boundary condition for: $ y\rightarrow\infty $\\
	Becomes the boundary condition for: $ Y\rightarrow\infty$\\
	This equation can be broken into three parts:
	\subsubsection{u}
	\begin{gather*}
		\eta\pd{u}{y}\rightarrow\tau_s \tag{5a} \\
		\left[\eta\right]\mu\frac{\left[u\right]}{\left[z\right]}\pd{U}{Y}\rightarrow\tau_s\\
		\mu\pd{U}{Y}\rightarrow\frac{\tau_s\left[z\right]}{\left[u\right]\left[\eta\right]} \tag{5a$ ' $}
	\end{gather*}
	\subsubsection{v}
	\begin{gather*}
		\pd{v}{z} \rightarrow 0 \tag{5b} \\
		\pd{V}{Z} \rightarrow 0 \tag{25b}
	\end{gather*}
	\subsubsection{w}
	\begin{gather*}
		w \rightarrow 0 \tag{5c} \\
		W \rightarrow 0 \tag{25c}
	\end{gather*}
	\subsection{6 $ \rightarrow $ 26}
	Boundary condition for: $ y\rightarrow-\infty $\\
	Becomes the boundary condition for: $ Y\rightarrow-\infty$\\
	This equation can be broken into three parts:
	\subsubsection{u}
	\begin{gather*}
		u \rightarrow 0 \tag{6a} \\
		U \rightarrow 0 \tag{26a}
	\end{gather*}
	\subsubsection{v}
	\begin{gather*}
		v \rightarrow \frac{n+2}{n+1}\frac{q_r}{h_s}\left[1-\left(1-\frac{z}{h_s}\right)^{n+1}\right] \tag{6b} \\
		v \rightarrow \frac{n+2}{n+1}\frac{q_r}{h_s}\left[1-\left(1-\frac{\left[z\right]Z}{h_s}\right)^{n+1}\right] \tag{6b'}
	\end{gather*}
	\subsubsection{w}
	\begin{gather*}
		w \rightarrow 0 \tag{6c} \\
		W \rightarrow 0 \tag{26c}
	\end{gather*}
	\subsection{7 $ \rightarrow $ 28}
	Boundary condition for: $ z = 0 $\\
	Becomes the boundary condition for: $ Z = 0 $
	\begin{gather*}
		w = 0 \text{ at } z = 0 \tag{7} \\
		W = 0 \text{ at } Z = 0 \tag{28}
	\end{gather*}
	\subsection{8 $ \rightarrow $ 29}
	Boundary condition for: $ y > 0,\ z = 0 $\\
	Becomes the boundary condition for: $ Y > 0,\ Z = 0 $\\
	This equation can be broken into two parts:
	\subsubsection{u}
	\begin{gather*}
		\eta\pd{u}{z} = 0 \tag{8a} \\
		\left[\eta\right]\mu\frac{\left[u\right]}{\left[z\right]}\pd{U}{Z} = 0\\
		\mu\pd{U}{Z} = 0 \tag{29a}
	\end{gather*}
	\subsubsection{v}
	\begin{gather*}
		\eta\pd{v}{z} = 0 \tag{8b} \\
		\left[\eta\right]\mu\frac{\left[v\right]}{\left[z\right]}\pd{V}{Z} = 0\\
		\mu\pd{V}{Z} = 0 \tag{29b}
	\end{gather*}
	\subsection{9a $ \rightarrow $ 30a}
	No slip boundary condition for: $ y < 0,\ z = 0 $\\
	Becomes the no slip boundary condition for: $ Y < 0,\ Z = 0 $
	\begin{gather*}
		u = v = 0 \tag{9a} \\
		U = V = 0 \tag{30a}
	\end{gather*}
	\subsection{9b $ \rightarrow $ 30b}
	Subtemperate slip boundary condition for: $ y < 0,\ z = 0 $\\
	Becomes the subtemperate slip boundary condition for: $ Y < 0,\ Z = 0 $
	This equation can be broken into three parts:
	\subsubsection{$ \sqrt{u^2+v^2}>0 $, u}
	\begin{gather*}
		\eta\pd{u}{z} = \tau_c\frac{u}{\sqrt{u^2+v^2}} \tag{9b,I} \\
		\left[\eta\right]\mu\frac{\left[u\right]}{\left[z\right]}\pd{U}{Z} = \tau_c\frac{U}{\sqrt{U^2+\frac{\left[v\right]^2}{\left[u\right]^2}V^2}}\\
		\mu\pd{U}{Z} = \frac{\left[z\right]\tau_c}{\left[u\right]\left[\eta\right]}\frac{U}{\sqrt{U^2+\frac{\left[v\right]^2}{\left[u\right]^2}V^2}} \tag{9b',I}
	\end{gather*}
	\subsubsection{$ \sqrt{u^2+v^2}>0 $, v}
	\begin{gather*}
		\eta\pd{v}{z} = \tau_c\frac{v}{\sqrt{u^2+v^2}} \tag{9b,II} \\
		\left[\eta\right]\mu\frac{\left[v\right]}{\left[z\right]}\pd{V}{Z} = \tau_c\frac{\left[v\right]}{\left[u\right]}\frac{V}{\sqrt{U^2+\frac{\left[v\right]^2}{\left[u\right]^2}V^2}}\\
		\mu\pd{V}{Z} = \frac{\left[z\right]\tau_c}{\left[u\right]\left[\eta\right]}\frac{V}{\sqrt{U^2+\frac{\left[v\right]^2}{\left[u\right]^2}V^2}} \tag{9b',II}
	\end{gather*}
	\subsubsection{$ \sqrt{u^2+v^2}=0 $}
	\begin{gather*}
		\sqrt{\left(\eta\pd{u}{z}\right)^2 + \left(\eta\pd{v}{z}\right)^2}\leq\tau_c \tag{9b,III} \\
		\frac{\left[\eta\right]\left[u\right]}{\left[z\right]}\sqrt{\left(\mu\pd{U}{Z}\right)^2+\left(\mu\frac{\left[v\right]}{\left[u\right]}\pd{V}{Z}\right)^2}\leq\tau_c\\
		\sqrt{\left(\mu\pd{U}{Z}\right)^2+\frac{\left[v\right]^2}{\left[u\right]^2}\left(\mu\pd{V}{Z}\right)^2}\leq\frac{\left[z\right]\tau_c}{\left[u\right]\left[\eta\right]} \tag{9b',III}
	\end{gather*}
	\subsection{10 $ \rightarrow $ 27}
	Boundary condition for: $ z = h_s $\\
	Becomes the boundary condition for: $ Z = 1 $\\
	This equation can be broken into four parts:
	\subsubsection{u}
	\begin{gather*}
		\eta\pd{u}{z} = 0 \tag{10a} \\
		\mu\pd{U}{Z} = 0 \tag{27a}
	\end{gather*}
	\subsubsection{v}
	\begin{gather*}
		\eta\pd{v}{z} = 0 \tag{10b} \\
		\mu\pd{V}{Z} = 0 \tag{27b}
	\end{gather*}
	\subsubsection{w}
	\begin{gather*}
		w = 0 \tag{10c} \\
		W = 0 \tag{27c}
	\end{gather*}
	\subsubsection{p}
	\begin{gather*}
		2\eta\pd{w}{z} - p + \rho g s' = 0 \tag{10d} \\
		2\left[\eta\right]\mu\frac{\left[v\right]}{\left[z\right]}\pd{W}{Z} - \left[p\right]P + \rho g\left[s'\right]S' = 0\\
		2\mu\pd{W}{Z} - \frac{\left[z\right]\left[p\right]}{\left[\eta\right]\left[v\right]}P + \frac{\rho g \left[s'\right]\left[z\right]}{\left[\eta\right]\left[v\right]}S' = 0 \tag{10d'}
	\end{gather*}
	
	\section{Finding Scales and Resolving the Primes}
	\subsection{5a'}
	This equation gives the first two scales:
	\begin{gather*}
		\left[z\right] = h_s\\
		\tau_s = \frac{\left[u\right]\left[\eta\right]}{\left[z\right]} = \frac{\left[u\right]\left[\eta\right]}{h_s}
	\end{gather*}
	Which gives the final form:
	\begin{equation*}
		\mu\pd{U}{Y}\rightarrow 1 \tag{25a}
	\end{equation*}
	
\end{document}